PropositionalLogic/ProofTheory/RewriteClass.v
@@ -2,9 +2,9 @@ Require Import Coq.Classes.Morphisms.
 Require Import Coq.Classes.RelationClasses.
 Require Import Logic.lib.Coqlib.
 Require Import Logic.GeneralLogic.Base.
+Require Import Logic.GeneralLogic.ProofTheory.BasicSequentCalculus.
 Require Import Logic.MinimunLogic.Syntax.
-Require Import Logic.MinimunLogic.ProofTheory.Normal.
-Require Import Logic.MinimunLogic.ProofTheory.Minimun.
+Require Import Logic.MinimunLogic.ProofTheory.Minimun2.
 Require Import Logic.MinimunLogic.ProofTheory.RewriteClass.
 Require Import Logic.PropositionalLogic.Syntax.
 Require Import Logic.PropositionalLogic.ProofTheory.Intuitionistic.
@@ -13,7 +13,19 @@ Local Open Scope logic_base.
 Local Open Scope syntax.
 Import PropositionalLanguageNotation.
 
-Instance andp_proper_impp {L: Language} {nL: NormalLanguage L} {pL: PropositionalLanguage L} {Gamma: ProofTheory L} {nGamma: NormalProofTheory L Gamma} {mpGamma: MinimunPropositionalLogic L Gamma} {ipGamma: IntuitionisticPropositionalLogic L Gamma}: Proper ((fun x y => |-- impp x y) ==> (fun x y => |-- impp x y) ==> (fun x y => |-- impp x y)) andp.
+Section RewriteClass.
+
+Context {L: Language}
+        {minL: MinimunLanguage L}
+        {pL: PropositionalLanguage L}
+        {Gamma: ProofTheory L}
+        {SC: NormalSequentCalculus L Gamma}
+        {bSC: BasicSequentCalculus L Gamma}
+        {minSC: MinimunSequentCalculus L Gamma}
+        {minAX: MinimunAxiomatization L Gamma}
+        {ipGamma: IntuitionisticPropositionalLogic L Gamma}.
+
+Instance andp_proper_impp: Proper ((fun x y => |-- impp x y) ==> (fun x y => |-- impp x y) ==> (fun x y => |-- impp x y)) andp.
 Proof.
   hnf; intros x1 x2 ?.
   hnf; intros y1 y2 ?.
@@ -29,7 +41,7 @@ Proof.
   apply deduction_andp_intros; auto.
 Qed.
 
-Instance orp_proper_impp {L: Language} {nL: NormalLanguage L} {pL: PropositionalLanguage L} {Gamma: ProofTheory L} {nGamma: NormalProofTheory L Gamma} {mpGamma: MinimunPropositionalLogic L Gamma} {ipGamma: IntuitionisticPropositionalLogic L Gamma}: Proper ((fun x y => |-- impp x y) ==> (fun x y => |-- impp x y) ==> (fun x y => |-- impp x y)) orp.
+Instance orp_proper_impp: Proper ((fun x y => |-- impp x y) ==> (fun x y => |-- impp x y) ==> (fun x y => |-- impp x y)) orp.
 Proof.
   hnf; intros x1 x2 ?.
   hnf; intros y1 y2 ?.
@@ -41,7 +53,7 @@ Proof.
     apply derivable_orp_intros2.
 Qed.
 
-Instance negp_proper_impp {L: Language} {nL: NormalLanguage L} {pL: PropositionalLanguage L} {Gamma: ProofTheory L} {nGamma: NormalProofTheory L Gamma} {mpGamma: MinimunPropositionalLogic L Gamma} {ipGamma: IntuitionisticPropositionalLogic L Gamma}: Proper ((fun x y => |-- impp x y) --> (fun x y => |-- impp x y)) negp.
+Instance negp_proper_impp: Proper ((fun x y => |-- impp x y) --> (fun x y => |-- impp x y)) negp.
 Proof.
   hnf; intros x1 x2 ?.
   unfold negp.
@@ -49,9 +61,9 @@ Proof.
   apply provable_impp_refl.
 Qed.
 
-Instance provable_iffp_rewrite {L: Language} {nL: NormalLanguage L} {pL: PropositionalLanguage L} {Gamma: ProofTheory L} {nGamma: NormalProofTheory L Gamma} {mpGamma: MinimunPropositionalLogic L Gamma} {ipGamma: IntuitionisticPropositionalLogic L Gamma}: RewriteRelation (fun x y => |-- x <--> y).
+Instance provable_iffp_rewrite: RewriteRelation (fun x y => |-- x <--> y).
 
-Instance provable_iffp_equiv {L: Language} {nL: NormalLanguage L} {pL: PropositionalLanguage L} {Gamma: ProofTheory L} {nGamma: NormalProofTheory L Gamma} {mpGamma: MinimunPropositionalLogic L Gamma} {ipGamma: IntuitionisticPropositionalLogic L Gamma}: Equivalence (fun x y => |-- x <--> y).
+Instance provable_iffp_equiv: Equivalence (fun x y => |-- x <--> y).
 Proof.
   constructor.
   + hnf; intros.
@@ -71,7 +83,7 @@ Proof.
     apply deduction_andp_intros; eapply deduction_impp_trans; eauto.
 Qed.
 
-Instance provable_proper_iffp {L: Language} {nL: NormalLanguage L} {pL: PropositionalLanguage L} {Gamma: ProofTheory L} {nGamma: NormalProofTheory L Gamma} {mpGamma: MinimunPropositionalLogic L Gamma} {ipGamma: IntuitionisticPropositionalLogic L Gamma} : Proper ((fun x y => |-- x <--> y) ==> iff) provable.
+Instance provable_proper_iffp : Proper ((fun x y => |-- x <--> y) ==> iff) provable.
 Proof.
   intros.
   hnf; intros.
@@ -84,7 +96,7 @@ Proof.
   eapply deduction_modus_ponens; eauto.
 Qed.
 
-Instance derivable_proper_iffp {L: Language} {nL: NormalLanguage L} {pL: PropositionalLanguage L} {Gamma: ProofTheory L} {nGamma: NormalProofTheory L Gamma} {mpGamma: MinimunPropositionalLogic L Gamma} {ipGamma: IntuitionisticPropositionalLogic L Gamma} : Proper (eq ==> (fun x y => |-- x <--> y) ==> iff) derivable.
+Instance derivable_proper_iffp : Proper (eq ==> (fun x y => |-- x <--> y) ==> iff) derivable.
 Proof.
   hnf; intros Phi Phi' ?; subst Phi'.
   hnf; intros x1 x2 ?.
@@ -95,7 +107,7 @@ Proof.
   eapply deduction_modus_ponens; eauto.
 Qed.
 
-Instance impp_proper_iffp {L: Language} {nL: NormalLanguage L} {pL: PropositionalLanguage L} {Gamma: ProofTheory L} {nGamma: NormalProofTheory L Gamma} {mpGamma: MinimunPropositionalLogic L Gamma} {ipGamma: IntuitionisticPropositionalLogic L Gamma} : Proper ((fun x y => |-- x <--> y) ==> (fun x y => |-- x <--> y) ==> (fun x y => |-- x <--> y)) impp.
+Instance impp_proper_iffp : Proper ((fun x y => |-- x <--> y) ==> (fun x y => |-- x <--> y) ==> (fun x y => |-- x <--> y)) impp.
 Proof.
   hnf; intros x1 x2 ?.
   hnf; intros y1 y2 ?.
@@ -115,7 +127,7 @@ Proof.
   + apply impp_proper_impp; auto.
 Qed.
 
-Instance andp_proper_iffp {L: Language} {nL: NormalLanguage L} {pL: PropositionalLanguage L} {Gamma: ProofTheory L} {nGamma: NormalProofTheory L Gamma} {mpGamma: MinimunPropositionalLogic L Gamma} {ipGamma: IntuitionisticPropositionalLogic L Gamma}: Proper ((fun x y => |-- x <--> y) ==> (fun x y => |-- x <--> y) ==> (fun x y => |-- x <--> y)) andp.
+Instance andp_proper_iffp: Proper ((fun x y => |-- x <--> y) ==> (fun x y => |-- x <--> y) ==> (fun x y => |-- x <--> y)) andp.
 Proof.
   hnf; intros x1 x2 ?.
   hnf; intros y1 y2 ?.
@@ -135,7 +147,7 @@ Proof.
   + apply andp_proper_impp; auto.
 Qed.
 
-Instance orp_proper_iffp {L: Language} {nL: NormalLanguage L} {pL: PropositionalLanguage L} {Gamma: ProofTheory L} {nGamma: NormalProofTheory L Gamma} {mpGamma: MinimunPropositionalLogic L Gamma} {ipGamma: IntuitionisticPropositionalLogic L Gamma}: Proper ((fun x y => |-- x <--> y) ==> (fun x y => |-- x <--> y) ==> (fun x y => |-- x <--> y)) orp.
+Instance orp_proper_iffp: Proper ((fun x y => |-- x <--> y) ==> (fun x y => |-- x <--> y) ==> (fun x y => |-- x <--> y)) orp.
 Proof.
   hnf; intros x1 x2 ?.
   hnf; intros y1 y2 ?.
@@ -155,7 +167,7 @@ Proof.
   + apply orp_proper_impp; auto.
 Qed.
 
-Instance iffp_proper_iffp {L: Language} {nL: NormalLanguage L} {pL: PropositionalLanguage L} {Gamma: ProofTheory L} {nGamma: NormalProofTheory L Gamma} {mpGamma: MinimunPropositionalLogic L Gamma} {ipGamma: IntuitionisticPropositionalLogic L Gamma}: Proper ((fun x y => |-- x <--> y) ==> (fun x y => |-- x <--> y) ==> (fun x y => |-- x <--> y)) iffp.
+Instance iffp_proper_iffp: Proper ((fun x y => |-- x <--> y) ==> (fun x y => |-- x <--> y) ==> (fun x y => |-- x <--> y)) iffp.
 Proof.
   hnf; intros x1 x2 ?.
   hnf; intros y1 y2 ?.
@@ -164,10 +176,17 @@ Proof.
   apply provable_iffp_refl.
 Qed.
 
-Instance negp_proper_iffp {L: Language} {nL: NormalLanguage L} {pL: PropositionalLanguage L} {Gamma: ProofTheory L} {nGamma: NormalProofTheory L Gamma} {mpGamma: MinimunPropositionalLogic L Gamma} {ipGamma: IntuitionisticPropositionalLogic L Gamma}: Proper ((fun x y => |-- x <--> y) ==> (fun x y => |-- x <--> y)) negp.
+Instance negp_proper_iffp: Proper ((fun x y => |-- x <--> y) ==> (fun x y => |-- x <--> y)) negp.
 Proof.
   hnf; intros x1 x2 ?.
   unfold negp.
   apply impp_proper_iffp; auto.
   apply provable_iffp_refl.
 Qed.
+
+End RewriteClass.
+
+Existing Instances andp_proper_impp orp_proper_impp negp_proper_impp
+                   provable_iffp_rewrite provable_iffp_equiv
+                   provable_proper_iffp derivable_proper_iffp
+                   impp_proper_iffp andp_proper_iffp orp_proper_iffp iffp_proper_iffp negp_proper_iffp.
